Morpho/Proofs/YulRewriteProofs.lean
@@ -100,6 +100,496 @@ axiom semantic_eq :
 
 end market_params_hash
 
+namespace abi_decode_bool
+
+axiom semantic_eq :
+  RewriteProofObligation
+    "rewrite.abi_decode_bool.semantic_eq"
+    "abi_decode_bool-canonicalization"
+    "abi_decode_bool"
+
+end abi_decode_bool
+
+namespace abi_decode_bytes
+
+axiom semantic_eq :
+  RewriteProofObligation
+    "rewrite.abi_decode_bytes.semantic_eq"
+    "abi_decode_bytes-canonicalization"
+    "abi_decode_bytes"
+
+end abi_decode_bytes
+
+namespace abi_decode_struct
+
+axiom semantic_eq :
+  RewriteProofObligation
+    "rewrite.abi_decode_struct.semantic_eq"
+    "abi_decode_struct-canonicalization"
+    "abi_decode_struct"
+
+end abi_decode_struct
+
+namespace abi_encode_address
+
+axiom semantic_eq :
+  RewriteProofObligation
+    "rewrite.abi_encode_address.semantic_eq"
+    "abi_encode_address-canonicalization"
+    "abi_encode_address"
+
+end abi_encode_address
+
+namespace abi_encode_uint256
+
+axiom semantic_eq :
+  RewriteProofObligation
+    "rewrite.abi_encode_uint256.semantic_eq"
+    "abi_encode_uint256-canonicalization"
+    "abi_encode_uint256"
+
+end abi_encode_uint256
+
+namespace array_allocation_size
+
+axiom semantic_eq :
+  RewriteProofObligation
+    "rewrite.array_allocation_size.semantic_eq"
+    "array_allocation_size-canonicalization"
+    "array_allocation_size"
+
+end array_allocation_size
+
+namespace checked_div
+
+axiom semantic_eq :
+  RewriteProofObligation
+    "rewrite.checked_div.semantic_eq"
+    "checked_div-canonicalization"
+    "checked_div"
+
+end checked_div
+
+namespace checked_mul
+
+axiom semantic_eq :
+  RewriteProofObligation
+    "rewrite.checked_mul.semantic_eq"
+    "checked_mul-canonicalization"
+    "checked_mul"
+
+end checked_mul
+
+namespace checked_sub
+
+axiom semantic_eq :
+  RewriteProofObligation
+    "rewrite.checked_sub.semantic_eq"
+    "checked_sub-canonicalization"
+    "checked_sub"
+
+end checked_sub
+
+namespace extract_returndata
+
+axiom semantic_eq :
+  RewriteProofObligation
+    "rewrite.extract_returndata.semantic_eq"
+    "extract_returndata-canonicalization"
+    "extract_returndata"
+
+end extract_returndata
+
+namespace finalize_allocation
+
+axiom semantic_eq :
+  RewriteProofObligation
+    "rewrite.finalize_allocation.semantic_eq"
+    "finalize_allocation-canonicalization"
+    "finalize_allocation"
+
+end finalize_allocation
+
+namespace fun_helpers
+
+axiom semantic_eq :
+  RewriteProofObligation
+    "rewrite.fun_helpers.semantic_eq"
+    "fun-canonicalization"
+    "fun"
+
+end fun_helpers
+
+namespace increment_uint256
+
+axiom semantic_eq :
+  RewriteProofObligation
+    "rewrite.increment_uint256.semantic_eq"
+    "increment_uint256-canonicalization"
+    "increment_uint256"
+
+end increment_uint256
+
+namespace internal_modifier_onlyowner
+
+axiom semantic_eq :
+  RewriteProofObligation
+    "rewrite.internal_modifier_onlyowner.semantic_eq"
+    "internal_modifier_onlyowner-canonicalization"
+    "internal___modifier_onlyOwner"
+
+end internal_modifier_onlyowner
+
+namespace internal_internal_domain_separator
+
+axiom semantic_eq :
+  RewriteProofObligation
+    "rewrite.internal_internal_domain_separator.semantic_eq"
+    "internal_internal_domain_separator-canonicalization"
+    "internal_internal_DOMAIN_SEPARATOR"
+
+end internal_internal_domain_separator
+
+namespace internal_internal_accrueinterest
+
+axiom semantic_eq :
+  RewriteProofObligation
+    "rewrite.internal_internal_accrueinterest.semantic_eq"
+    "internal_internal_accrueinterest-canonicalization"
+    "internal_internal_accrueInterest"
+
+end internal_internal_accrueinterest
+
+namespace internal_internal_borrow
+
+axiom semantic_eq :
+  RewriteProofObligation
+    "rewrite.internal_internal_borrow.semantic_eq"
+    "internal_internal_borrow-canonicalization"
+    "internal_internal_borrow"
+
+end internal_internal_borrow
+
+namespace internal_internal_createmarket
+
+axiom semantic_eq :
+  RewriteProofObligation
+    "rewrite.internal_internal_createmarket.semantic_eq"
+    "internal_internal_createmarket-canonicalization"
+    "internal_internal_createMarket"
+
+end internal_internal_createmarket
+
+namespace internal_internal_enableirm
+
+axiom semantic_eq :
+  RewriteProofObligation
+    "rewrite.internal_internal_enableirm.semantic_eq"
+    "internal_internal_enableirm-canonicalization"
+    "internal_internal_enableIrm"
+
+end internal_internal_enableirm
+
+namespace internal_internal_enablelltv
+
+axiom semantic_eq :
+  RewriteProofObligation
+    "rewrite.internal_internal_enablelltv.semantic_eq"
+    "internal_internal_enablelltv-canonicalization"
+    "internal_internal_enableLltv"
+
+end internal_internal_enablelltv
+
+namespace internal_internal_fee
+
+axiom semantic_eq :
+  RewriteProofObligation
+    "rewrite.internal_internal_fee.semantic_eq"
+    "internal_internal_fee-canonicalization"
+    "internal_internal_fee"
+
+end internal_internal_fee
+
+namespace internal_internal_feerecipient
+
+axiom semantic_eq :
+  RewriteProofObligation
+    "rewrite.internal_internal_feerecipient.semantic_eq"
+    "internal_internal_feerecipient-canonicalization"
+    "internal_internal_feeRecipient"
+
+end internal_internal_feerecipient
+
+namespace internal_internal_flashloan
+
+axiom semantic_eq :
+  RewriteProofObligation
+    "rewrite.internal_internal_flashloan.semantic_eq"
+    "internal_internal_flashloan-canonicalization"
+    "internal_internal_flashLoan"
+
+end internal_internal_flashloan
+
+namespace internal_internal_idtomarketparams
+
+axiom semantic_eq :
+  RewriteProofObligation
+    "rewrite.internal_internal_idtomarketparams.semantic_eq"
+    "internal_internal_idtomarketparams-canonicalization"
+    "internal_internal_idToMarketParams"
+
+end internal_internal_idtomarketparams
+
+namespace internal_internal_isauthorized
+
+axiom semantic_eq :
+  RewriteProofObligation
+    "rewrite.internal_internal_isauthorized.semantic_eq"
+    "internal_internal_isauthorized-canonicalization"
+    "internal_internal_isAuthorized"
+
+end internal_internal_isauthorized
+
+namespace internal_internal_isirmenabled
+
+axiom semantic_eq :
+  RewriteProofObligation
+    "rewrite.internal_internal_isirmenabled.semantic_eq"
+    "internal_internal_isirmenabled-canonicalization"
+    "internal_internal_isIrmEnabled"
+
+end internal_internal_isirmenabled
+
+namespace internal_internal_islltvenabled
+
+axiom semantic_eq :
+  RewriteProofObligation
+    "rewrite.internal_internal_islltvenabled.semantic_eq"
+    "internal_internal_islltvenabled-canonicalization"
+    "internal_internal_isLltvEnabled"
+
+end internal_internal_islltvenabled
+
+namespace internal_internal_lastupdate
+
+axiom semantic_eq :
+  RewriteProofObligation
+    "rewrite.internal_internal_lastupdate.semantic_eq"
+    "internal_internal_lastupdate-canonicalization"
+    "internal_internal_lastUpdate"
+
+end internal_internal_lastupdate
+
+namespace internal_internal_liquidate
+
+axiom semantic_eq :
+  RewriteProofObligation
+    "rewrite.internal_internal_liquidate.semantic_eq"
+    "internal_internal_liquidate-canonicalization"
+    "internal_internal_liquidate"
+
+end internal_internal_liquidate
+
+namespace internal_internal_market
+
+axiom semantic_eq :
+  RewriteProofObligation
+    "rewrite.internal_internal_market.semantic_eq"
+    "internal_internal_market-canonicalization"
+    "internal_internal_market"
+
+end internal_internal_market
+
+namespace internal_internal_nonce
+
+axiom semantic_eq :
+  RewriteProofObligation
+    "rewrite.internal_internal_nonce.semantic_eq"
+    "internal_internal_nonce-canonicalization"
+    "internal_internal_nonce"
+
+end internal_internal_nonce
+
+namespace internal_internal_owner
+
+axiom semantic_eq :
+  RewriteProofObligation
+    "rewrite.internal_internal_owner.semantic_eq"
+    "internal_internal_owner-canonicalization"
+    "internal_internal_owner"
+
+end internal_internal_owner
+
+namespace internal_internal_position
+
+axiom semantic_eq :
+  RewriteProofObligation
+    "rewrite.internal_internal_position.semantic_eq"
+    "internal_internal_position-canonicalization"
+    "internal_internal_position"
+
+end internal_internal_position
+
+namespace internal_internal_repay
+
+axiom semantic_eq :
+  RewriteProofObligation
+    "rewrite.internal_internal_repay.semantic_eq"
+    "internal_internal_repay-canonicalization"
+    "internal_internal_repay"
+
+end internal_internal_repay
+
+namespace internal_internal_setauthorization
+
+axiom semantic_eq :
+  RewriteProofObligation
+    "rewrite.internal_internal_setauthorization.semantic_eq"
+    "internal_internal_setauthorization-canonicalization"
+    "internal_internal_setAuthorization"
+
+end internal_internal_setauthorization
+
+namespace internal_internal_setauthorizationwithsig
+
+axiom semantic_eq :
+  RewriteProofObligation
+    "rewrite.internal_internal_setauthorizationwithsig.semantic_eq"
+    "internal_internal_setauthorizationwithsig-canonicalization"
+    "internal_internal_setAuthorizationWithSig"
+
+end internal_internal_setauthorizationwithsig
+
+namespace internal_internal_setfee
+
+axiom semantic_eq :
+  RewriteProofObligation
+    "rewrite.internal_internal_setfee.semantic_eq"
+    "internal_internal_setfee-canonicalization"
+    "internal_internal_setFee"
+
+end internal_internal_setfee
+
+namespace internal_internal_setfeerecipient
+
+axiom semantic_eq :
+  RewriteProofObligation
+    "rewrite.internal_internal_setfeerecipient.semantic_eq"
+    "internal_internal_setfeerecipient-canonicalization"
+    "internal_internal_setFeeRecipient"
+
+end internal_internal_setfeerecipient
+
+namespace internal_internal_setowner
+
+axiom semantic_eq :
+  RewriteProofObligation
+    "rewrite.internal_internal_setowner.semantic_eq"
+    "internal_internal_setowner-canonicalization"
+    "internal_internal_setOwner"
+
+end internal_internal_setowner
+
+namespace internal_internal_supply
+
+axiom semantic_eq :
+  RewriteProofObligation
+    "rewrite.internal_internal_supply.semantic_eq"
+    "internal_internal_supply-canonicalization"
+    "internal_internal_supply"
+
+end internal_internal_supply
+
+namespace internal_internal_supplycollateral
+
+axiom semantic_eq :
+  RewriteProofObligation
+    "rewrite.internal_internal_supplycollateral.semantic_eq"
+    "internal_internal_supplycollateral-canonicalization"
+    "internal_internal_supplyCollateral"
+
+end internal_internal_supplycollateral
+
+namespace internal_internal_totalborrowassets
+
+axiom semantic_eq :
+  RewriteProofObligation
+    "rewrite.internal_internal_totalborrowassets.semantic_eq"
+    "internal_internal_totalborrowassets-canonicalization"
+    "internal_internal_totalBorrowAssets"
+
+end internal_internal_totalborrowassets
+
+namespace internal_internal_totalborrowshares
+
+axiom semantic_eq :
+  RewriteProofObligation
+    "rewrite.internal_internal_totalborrowshares.semantic_eq"
+    "internal_internal_totalborrowshares-canonicalization"
+    "internal_internal_totalBorrowShares"
+
+end internal_internal_totalborrowshares
+
+namespace internal_internal_totalsupplyassets
+
+axiom semantic_eq :
+  RewriteProofObligation
+    "rewrite.internal_internal_totalsupplyassets.semantic_eq"
+    "internal_internal_totalsupplyassets-canonicalization"
+    "internal_internal_totalSupplyAssets"
+
+end internal_internal_totalsupplyassets
+
+namespace internal_internal_totalsupplyshares
+
+axiom semantic_eq :
+  RewriteProofObligation
+    "rewrite.internal_internal_totalsupplyshares.semantic_eq"
+    "internal_internal_totalsupplyshares-canonicalization"
+    "internal_internal_totalSupplyShares"
+
+end internal_internal_totalsupplyshares
+
+namespace internal_internal_withdraw
+
+axiom semantic_eq :
+  RewriteProofObligation
+    "rewrite.internal_internal_withdraw.semantic_eq"
+    "internal_internal_withdraw-canonicalization"
+    "internal_internal_withdraw"
+
+end internal_internal_withdraw
+
+namespace internal_internal_withdrawcollateral
+
+axiom semantic_eq :
+  RewriteProofObligation
+    "rewrite.internal_internal_withdrawcollateral.semantic_eq"
+    "internal_internal_withdrawcollateral-canonicalization"
+    "internal_internal_withdrawCollateral"
+
+end internal_internal_withdrawcollateral
+
+namespace require_helper_string
+
+axiom semantic_eq :
+  RewriteProofObligation
+    "rewrite.require_helper_string.semantic_eq"
+    "require_helper_string-canonicalization"
+    "require_helper_string"
+
+end require_helper_string
+
+namespace update_storage_value
+
+axiom semantic_eq :
+  RewriteProofObligation
+    "rewrite.update_storage_value.semantic_eq"
+    "update_storage_value-canonicalization"
+    "update_storage_value"
+
+end update_storage_value
+
 end rewrite
 
 end Morpho.Proofs.YulRewriteProofs
